Question 4 completeeeeeeeeeeeeeeeeeeeeeeeeeeeeeeeeeeeeeeeeeeeeeeeeeeeeeeeeeeeeeeeeeeee

ex2/imp.v
@@ -1,6 +1,5 @@
 Set Implicit Arguments.
 
-
 Inductive var := a | b | n | x | y.
 
 Definition op := nat -> nat -> nat.
@@ -44,3 +43,277 @@ Definition euclid_body :=
         (if_then_else (expr_op $a gt01 $b)
                       (assign a (expr_op $a sub $b))
                       (assign b (expr_op $b sub $a))).
+                      
+                      
+(* ====== Q4 ====== *)
+
+Inductive gcd : nat -> nat -> nat -> Prop :=
+| base   : forall z, gcd z z z
+| step_a : forall a b z, gcd a b z -> gcd (a + b) b z
+| step_b : forall a b z, gcd a b z -> gcd a (a + b) z.
+
+Section ReflexiveTransitiveClosureDef.
+
+  Variable D : Set.
+  Variable R : D -> D -> Prop.
+
+  Inductive tc : D -> D -> Prop :=
+    tc_refl : forall s, tc s s
+  | tc_step : forall s u t, R s u -> tc u t -> tc s t.
+    
+End ReflexiveTransitiveClosureDef.
+
+(*Definition var_eq_dec (v1 v2 : var) : {v1 = v2} + {v1 <> v2}.
+Proof.
+  decide equality.
+Defined.*)
+
+Definition eq_var (v1 v2 : var) : bool :=
+  match v1, v2 with
+  | a, a => true
+  | b, b => true
+  | n, n => true
+  | x, x => true
+  | y, y => true
+  | _, _ => false
+  end.
+
+Inductive sos : (state * cmd) -> (state * cmd) -> Prop :=
+| sos_asn : forall s v e,
+    sos (s, assign v e) 
+    ((fun v' : var => if eq_var v v' then sem e s else s v'), skip)
+    
+| sos_seq : forall s s' c1 c1' c2,
+    sos (s, c1) (s', c1') ->
+    sos (s, (seq c1 c2)) (s', (seq c1' c2))
+    
+| sos_skp : forall s c2,
+    sos (s, seq skip c2) (s, c2)
+
+| sos_if_true: forall s e c1 c2,
+    sem e s <> 0 ->
+    sos (s, if_then_else e c1 c2) (s, c1)
+
+| sos_if_false: forall s e c1 c2,
+    sem e s = 0 ->
+    sos (s, if_then_else e c1 c2) (s, c2)
+
+| sos_while_true: forall s e c,
+    sem e s <> 0 ->
+    sos (s, while e c) (s, seq c (while e c))
+
+| sos_while_false: forall s e c,
+    sem e s = 0 ->
+    sos (s, while e c) (s, skip)
+
+| sos_assume_true: forall s e,
+    sem e s <> 0 ->
+    sos (s, assume e) (s, skip)
+.
+      
+Definition step : state -> state -> Prop := 
+  fun s s' => tc sos (s, euclid_body) (s', skip).
+
+Lemma tc_trans : forall (D : Set) (R : D -> D -> Prop) (x y z : D),
+                 tc R x y -> tc R y z -> tc R x z.
+Proof.
+  intros D R x y z Hxy Hyz.
+  induction Hxy.
+  - apply Hyz.
+  - apply tc_step with u. 
+    + apply H.
+    + apply IHHxy.
+      apply Hyz.
+Qed.
+
+Lemma tc_inv : forall (D : Set) (R : D -> D -> Prop) (x z : D),
+               tc R x z -> x = z \/ exists y, R x y /\ tc R y z.
+Proof.
+  intros D R x z Hxz.
+  induction Hxz.
+  - left; reflexivity.
+  - right.
+    exists u.
+    split.
+    + apply H.
+    + apply Hxz.
+Qed.
+
+(* Case a => a > b *)
+(* Case a-a => Show that a becomes a-b *)
+Lemma case_a_a : forall s s', (s a) > (s b) -> step s s' -> (s' a) = (s a) - (s b).
+Proof.
+  intros s s' a_gr_b H.
+  inversion H; clear H.
+  
+  inversion H0; subst.
+  
+  inversion H7; subst. inversion H1; subst. inversion H.
+  - inversion H9; subst.
+  - subst. inversion H3; subst. inversion H4; subst.
+    + inversion H5; subst. inversion H6; subst. inversion H5; subst.
+      inversion H8; subst.
+      * firstorder.
+      * inversion H11.
+    + subst.
+      simpl in H12. unfold gt01, gt_dec in H12.
+      destruct lt_dec in H12.
+      * discriminate H12.
+      * firstorder.
+Qed.
+
+(* Case a-b => Show that b stay b *)
+Lemma case_a_b : forall s s', (s a) > (s b) -> step s s' -> (s' b) = (s b).
+Proof.
+  intros s s' a_gr_b H.
+  
+  inversion H; clear H; subst.
+  
+  inversion H0; subst.
+  inversion H5; subst.
+  inversion H1; subst.
+  inversion H; subst.
+  - inversion H9; subst.
+  - inversion H; subst.
+    inversion H3; subst.
+    inversion H4; subst.
+    + inversion H6; subst.
+      inversion H7; subst.
+      inversion H8; subst.
+      * reflexivity.
+      * inversion H9; subst.
+    + subst.
+      simpl in H12. unfold gt01, gt_dec in H12.
+      destruct lt_dec in H12.
+      * discriminate H12.
+      * firstorder.
+Qed.
+
+(* Case a => a <= b *)
+(* Case b-b => Show that b becomes b-a *)
+Lemma case_b_b : forall s s', (s a) <= (s b) -> step s s' -> (s' b) = (s b) - (s a).
+Proof.
+  intros s s' b_ge_a H.
+  assert (a_le_b : (s b) >= (s a)). { firstorder. }
+  inversion H; clear H.
+  
+  inversion H0; subst.
+  
+  inversion H7; subst. inversion H1; subst. inversion H.
+  - inversion H9; subst.
+  - subst. inversion H3; subst. inversion H4; subst.
+    + inversion H5; subst. inversion H6; subst. inversion H5; subst.
+      inversion H8; subst.
+      * simpl in H2, H12.
+        unfold gt01 in H12. unfold ne01 in H2.
+        destruct gt_dec in H12.
+        -- apply (le_ngt (s'0 a) (s'0 b)) in g.
+           contradiction.
+           firstorder.
+        -- contradiction.
+      * inversion H11.
+    + subst.
+      simpl in H12. unfold gt01, gt_dec in H12.
+      destruct lt_dec in H12.
+      * discriminate H12.
+      * inversion H5; subst. inversion H6; subst.
+        inversion H8; subst.
+        -- reflexivity.
+        -- inversion H9.
+Qed.
+
+(* Case b-a => Show that a stays a *)
+Lemma case_b_a : forall s s', (s a) <= (s b) -> step s s' -> (s' a) = (s a).
+Proof.
+  intros s s' b_ge_a H.
+  assert (a_le_b : (s b) >= (s a)). { firstorder. }
+  inversion H; clear H; subst.
+  
+  inversion H0; subst.
+  inversion H5; subst.
+  inversion H1; subst.
+  inversion H; subst.
+  - inversion H9; subst.
+  - inversion H; subst.
+    inversion H3; subst.
+    inversion H4; subst.
+    + inversion H6; subst.
+      inversion H7; subst.
+      simpl in H12. unfold gt01, gt_dec in H12.
+      destruct lt_dec in H12.
+      * apply (le_ngt (s'0 a) (s'0 b)) in l.
+        contradiction.
+        firstorder.
+      * contradiction.
+    + simpl in H12. unfold gt01, gt_dec in H12.
+      destruct lt_dec in H12.
+      * discriminate H12.
+      * subst. inversion H6; subst.
+        inversion H7; subst.
+        inversion H8; subst.
+        -- reflexivity.
+        -- inversion H9.
+Qed.
+
+Lemma step_modification_symmetry : forall s s', step s s' -> 
+                                   (s' b = s b) /\ (s a = s' a + s' b) 
+                                   \/
+                                   (s' a = s a) /\ (s b = s' a + s' b).
+Proof.
+  intros.
+  destruct (le_dec (s a) (s b)) as [Hle | Hgt].
+  - right.
+    assert (case_ba : s' a = s a). { apply case_b_a; assumption; assumption. }
+    assert (case_b : (s' a = s a) /\ (s b = s' a + s' b)).
+    {
+      split.
+      - assumption.
+      - rewrite case_ba. apply case_b_b in H. rewrite H. 
+        rewrite add_comm. symmetry. apply (Nat.sub_add (s a) (s b)). 
+        assumption. assumption.
+    }
+    assumption.
+  - left.
+    apply not_le in Hgt.
+    assert (case_ab : s' b = s b). { apply case_a_b; assumption; assumption. }
+    assert (case_a : (s' b = s b) /\ (s a = s' a + s' b)).
+    {
+      split.
+      - assumption.
+      - rewrite case_ab. apply case_a_a in H. rewrite H. 
+        symmetry. apply (Nat.sub_add (s b) (s a)). 
+        apply lt_le_incl in Hgt. assumption. assumption.
+    }
+    assumption.
+Qed.
+
+Lemma euclid_inv : forall s s' z,
+                   tc step s s' -> gcd (s' a) (s' b) z -> gcd (s a) (s b) z.
+Proof.
+  intros s s' z Step gcd'__s.
+  induction Step.
+  - assumption. 
+  - apply step_modification_symmetry in H.
+    destruct H.  
+    + destruct H. rewrite <- H in *. rewrite H0. apply step_a. 
+      apply IHStep. assumption.
+    + destruct H. rewrite <- H in *. rewrite H0. apply step_b.
+      apply IHStep. assumption.
+Qed.
+
+Theorem Correctness : forall (a0 b0 : nat) (s s' : state), 
+                      s a = a0 
+                      -> s b = b0 
+                      -> tc step s s' -> s' a = s' b
+                      -> gcd a0 b0 (s' a).
+Proof.
+  intros.
+  subst. 
+  assert (gcd (s' a) (s' b) (s' a)).
+    rewrite H2 in *. constructor.
+  rewrite H2 in *.
+  eapply euclid_inv.
+  apply H1.
+  rewrite H2 in *.
+  assumption.
+Qed.
